STLC: Add unit, prove exchange, work on preservation

LeanLam/STLC.lean
@@ -1,16 +1,38 @@
+import Aesop
+import Mathlib.Tactic
+
 namespace STLC
 
--- TATP p103
+-- de bruijn levels
+  -- raw
+  -- fin
+  -- dep
+-- de bruijn indicies
+  -- raw
+  -- fin
+  -- dep
+-- named
+  -- raw
+  -- dep
+-- locally nameless
+  -- raw
+  -- fin
+  -- dep
+-- phoas
+
+-- TAPL p103
 
 --- Syntax ---
 
 -- types
 inductive T
+| Unit : T
 | Arr : T → T → T
 deriving Repr, BEq, DecidableEq
 
 -- terms (de-bruijn)
-inductive t
+inductive t where
+| Unit : t
 | Var : Nat → t
 | Lam : T → t → t
 | App : t → t → t
@@ -18,12 +40,15 @@ deriving Repr, BEq, DecidableEq
 
 -- context
 
--- TODO: this representation is nice until you need exchange, figure out a better one
 abbrev Γ := List T
 
 --- Typing ---
 
 inductive types : Γ → t → T → Prop where
+| Unit
+  : ∀ ctx
+  , types ctx .Unit .Unit
+
 | Var
   : ∀ ctx n ty
   , ctx[n]? = some ty
@@ -44,6 +69,7 @@ inductive types : Γ → t → T → Prop where
 
 -- substitution
 def sub (depth : Nat) (new : t) : t → t
+| .Unit => .Unit
 | .Var idx =>
     if idx == depth then (inc new depth 0)
     else if idx > depth then .Var (idx - 1) -- decrement because we stripped a lambda
@@ -52,6 +78,7 @@ def sub (depth : Nat) (new : t) : t → t
 | .App f a => .App (sub depth new f) (sub depth new a)
 where
   inc (e : t) (amt : Nat) (depth : Nat) : t := match e with
+  | .Unit => .Unit
   | .Var i => if i ≥ depth then .Var (i + amt) else .Var i
   | .App f a => .App (inc f amt depth) (inc a amt depth)
   | .Lam ty body => .Lam ty (inc body amt (depth + 1))
@@ -59,20 +86,24 @@ where
 -- fully evaluated values
 def val : t → Prop
 | .Lam _ _ => True
+| .Unit => True
 | _ => False
 
 inductive eval : t → t → Prop where
 | App1
-  : eval t₁ t'₁
+  : ∀ t₁ t'₁ t₂
+  , eval t₁ t'₁
   → eval (.App t₁ t₂) (.App t'₁ t₂)
 
 | App2
-  : eval t₂ t'₂
+  : ∀ t₁ t₂ t'₂
+  , eval t₂ t'₂
   → val t₁
   → eval (.App t₁ t₂) (.App t₁ t'₂)
 
 | AppAbs
-  : val t₂
+  : ∀ t₁₂ t₂ T₁₁
+  , val t₂
   → eval (.App (.Lam T₁₁ t₁₂) t₂) (sub 0 t₂ t₁₂)
 
 --- Proofs ---
@@ -80,6 +111,7 @@ inductive eval : t → t → Prop where
 def closed : t → Prop := aux 0
 where
   aux (depth : Nat) (term : t) : Prop := match term with
+  | .Unit => True
   | .Var n => n < depth
   | .App f a => aux depth f ∧ aux depth a
   | .Lam _ body => aux (depth + 1) body
@@ -105,10 +137,78 @@ theorem app (h : types ctx (.App t₁ t₂) R) : ∃ T₁₁, types ctx t₁ (.A
 
 end inversions
 
+--- structural properties ---
+
+def t.swap (x y : Nat) : t → t
+| .Unit => .Unit
+| .App f a => .App (swap x y f) (swap x y a)
+| .Lam ty body => .Lam ty (swap (x + 1) (y + 1) body)
+| .Var idx =>
+  if idx == x then .Var y
+  else if idx == y then .Var x
+  else .Var idx
+
+def Γ.swap (x y : Nat) (ctx : Γ) : Γ :=
+  match ctx[x]?, ctx[y]? with
+  | some vx, some vy => ctx |> (List.set · x vy) |> (List.set · y vx)
+  | _, _ => ctx
+
+theorem exchange (x y : Nat) (ctx : Γ) (term : t) (ty : T) (hx : x < ctx.length) (hy : y < ctx.length)
+  : types ctx term ty → types (ctx.swap x y) (term.swap x y) ty := by
+    intro h
+    induction term generalizing ty ctx x y with
+    | Unit =>
+      unfold t.swap
+      unfold Γ.swap
+      simp_all
+      cases h with
+      | Unit =>
+        exact .Unit ((List.set ctx x ctx[y]).set y ctx[x])
+    | App f a ihf iha =>
+      cases h with
+      | App ctx t₁ t₂ T₁₁ T₁₂  hf ha =>
+        exact .App (ctx.swap x y) (f.swap x y) (a.swap x y) T₁₁ ty (ihf x y ctx (.Arr T₁₁ ty) hx hy hf) (iha x y ctx T₁₁ hx hy ha)
+    | Var i =>
+      unfold t.swap
+      split
+      case isTrue ht =>
+        unfold Γ.swap
+        simp_all
+        let ctx' := (List.set ctx x ctx[y]).set y ctx[x]
+        cases h with
+        | Var c i ty' hi => exact .Var ctx' y ty (by aesop)
+      case isFalse hf =>
+        unfold Γ.swap
+        simp_all
+        let ctx' := (List.set ctx x ctx[y]).set y ctx[x]
+        cases h with
+        | Var c i ty' hi =>
+          have hvar : t.Var (if i = y then x else i) = if i = y then t.Var x else t.Var i := by aesop
+          have skip_ne : ∀ (j a : Nat) (z : Type) (l : List z) (v : z),
+            ¬(j = a) → (List.set l a v)[j]? = l[j]? := by
+              intros j a z l v hneq
+              refine List.getElem?_set_ne ?h
+              exact Ne.symm hneq
+          have hlookup : ctx'[if i = y then x else i]? = some ty := by aesop
+          exact (hvar ▸ .Var ctx' (if i =y then x else i) ty hlookup)
+    | Lam ty body ihb =>
+      cases h with
+      | Abs ctx T₁ T₂ t₂ hb =>
+        have : ∀ (k : Nat) (α : Type) (l : List α) (hd : α), k < l.length → k + 1 < (hd :: l).length :=
+          by exact fun k α l hd a => Nat.add_lt_of_lt_sub a
+        have hswp : (Γ.swap (x + 1) (y + 1) (ty :: ctx)) = (ty :: Γ.swap x y ctx) := by
+          unfold Γ.swap; simp_all
+        have : types (ty :: Γ.swap x y ctx) (t.swap (x + 1) (y + 1) body) T₂ := by
+          exact (hswp ▸ ihb (x + 1) (y + 1) (ty :: ctx) T₂ (by aesop) (by aesop) hb)
+        exact .Abs (ctx.swap x y) ty T₂ (body.swap (x + 1) (y + 1)) this
+
+--- Type Soundness ---
+
 -- 9.3.4
 theorem cannonical_forms (term : t) (hv : val term) (ht : types ctx term (.Arr T₁ T₂)) : ∃ t₂, term = .Lam T₁ t₂ := by
   unfold val at hv
   cases term with
+  | Unit => contradiction
   | Var n => contradiction
   | App f a => contradiction
   | Lam Tₐ body =>
@@ -123,6 +223,7 @@ theorem cannonical_forms (term : t) (hv : val term) (ht : types ctx term (.Arr T
 theorem progress (term : t) (ty : T) : closed term → ctx = [] → types ctx term ty → val term ∨ ∃ term', eval term term' := by
   intros hclosed hempty htypes
   induction htypes with
+  | Unit => left; unfold val; simp
   | Var ih n => contradiction
   | Abs ctx' T₁ _ t₂ => left; simp [val]
   | App ctx' t₁ t₂ T₁₁ T₁₂ hf _ ihf iha =>
@@ -134,18 +235,84 @@ theorem progress (term : t) (ty : T) : closed term → ctx = [] → types ctx te
     | inr et1 =>
       right
       obtain ⟨t'₁, het1⟩ := et1
-      exact ⟨.App t'₁ t₂, .App1 het1⟩
+      exact ⟨.App t'₁ t₂, .App1 t₁ t'₁ t₂ het1⟩
     | inl vt1 => cases iha' with
       | inr et2 =>
         right
         obtain ⟨t'₂, het2⟩ := et2
-        exact ⟨.App t₁ t'₂, .App2 het2 vt1⟩
+        exact ⟨.App t₁ t'₂, .App2 t₁ t₂ t'₂ het2 vt1⟩
       | inl vt2 =>
         obtain ⟨t₁₂, ht12⟩ := cannonical_forms t₁ vt1 hf
         right
         rw [ht12]
-        exact ⟨sub 0 t₂ t₁₂, .AppAbs vt2⟩
+        exact ⟨sub 0 t₂ t₁₂, .AppAbs t₁₂ t₂ T₁₁ vt2⟩
 
-theorem preservation (ctx : Γ) (term : t) (term' : t) (ty : T) : types ctx term ty ∧ eval term term' → types ctx term' ty := by sorry
+theorem types_rfl (htypes : types ctx (t.Lam T₁₁ t₁₂) (.Arr T₁₂ ty)) : T₁₁ = T₁₂ := by
+  cases htypes with | Abs => aesop
+
+theorem sub_preserves (ctx : Γ) (S : T) (ty : T) (term : t) (s : t)
+  : types (S :: ctx) term ty → types ctx s S → types ctx (sub 0 s term) ty:= by
+    intros ht hs
+    induction hs with
+    | Unit ctx' => sorry
+    | Var ctx' n ty' hc =>
+      cases ht with
+      | Unit =>
+        simp_all [sub]
+        exact .Unit ctx'
+      | App ctx' t₁ t₂ T₁₁ T₁₂ hf ha =>
+        exact .App ctx' t₁ t₂ T₁₁ ty sorry sorry
+      | Abs => sorry
+      | Var ctx' i ty ha =>
+        simp_all [sub]
+        split
+        case isTrue htr =>
+          simp_all [sub.inc]
+          exact .Var ctx' n ty hc
+        case isFalse hfl =>
+          have : 0 < i := by omega
+          simp [this]
+          have : ctx'[i - 1]? = some ty := by
+            unfold getElem?
+            unfold getElem? at ha
+            unfold instGetElem?OfGetElemOfDecidable
+            unfold instGetElem?OfGetElemOfDecidable at ha
+            simp_all
+            obtain ⟨hl, hj⟩ := ha
+            have hlen : i - 1 < List.length ctx' := by omega
+            have hlen' : ∀ i α (a : α) l, i - 1 < l.length → i < (a :: l).length := by
+              intros i α a l hl
+              exact lt_of_tsub_lt_tsub_right hl
+            have helem (α : Type) (a : α) (l : List α) (hl' : i - 1 < l.length)
+              : (a :: l)[i]'(by aesop) = l[i - 1] := by
+                  sorry
+            have : ctx'[i - 1] = ty := by sorry
+            exact ⟨hlen, this⟩
+          exact .Var ctx' (i - 1) ty this
+    | Abs => sorry
+    | App => sorry
+
+theorem preservation (ctx : Γ) (term : t) (term' : t) (ty : T)
+  : types ctx term ty → eval term term' → types ctx term' ty := by
+    intros htypes heval
+    induction heval generalizing ty with
+    | App1 t₁ t'₁ t₂ he ih =>
+      cases htypes with
+      | App ctx t₁ t₂ T₁₁ T₁₂ hf ha =>
+        exact .App ctx t'₁ t₂ T₁₁ ty (ih (.Arr T₁₁ ty) hf) ha
+    | App2 t₁ t₂ t'₂ he hv ih =>
+      cases htypes with
+      | App ctx t₁ t₂ T₁₁ T₁₂ hf ha =>
+        exact .App ctx t₁ t'₂ T₁₁ ty hf (ih T₁₁ ha)
+    | AppAbs t₁₂ t₂ T₁₁ hv =>
+      cases htypes with
+      | App ctx t₁ t₂ T'₁₁ T₁₂ hf ha =>
+        -- TODO; T'₁₁ and T₁₁ should not be distinct vars
+        have : T₁₁ = T'₁₁ := by sorry
+        simp_all
+        cases hf with
+        | Abs ctx T₁ T₂ t₂ habs =>
+          unfold sub
+          sorry
 
 end STLC
